Based on the initial state, we know that `n_cases` is greater than 0, `i` is 0, `n` is an integer equal to `log2(n_cases - 1)`, and `power` is equal to `n`.

The `print` statement is `print(2 ** power)`. To determine what will be printed, we need to evaluate the expression `2 ** power`.

Since `power` is equal to `n`, we can substitute `n` into the expression: `2 ** n`.

Now, we need to find the value of `n`. We know that `n` is equal to `log2(n_cases - 1)`. This means that `n` is the base-2 logarithm of `n_cases - 1`.

Since `n_cases` is greater than 0, `n_cases - 1` is also greater than 0. Therefore, `log2(n_cases - 1)` is a well-defined value.

Let's assume that `n_cases` is a power of 2, say `n_cases = 2^k` for some integer `k`. Then, `n_cases - 1 = 2^k - 1`, and `log2(n_cases - 1) = log2(2^k - 1) = k - 1`.

So, in this case, `n = k - 1`.

Now, let's evaluate the expression `2 ** n`. Since `n = k - 1`, we have `2 ** n = 2 ** (k - 1) = 2^k / 2 = n_cases / 2`.

Therefore, the `print` statement will print the value of `n_cases / 2`.

Output: **n_cases / 2 (where n_cases is the value of n_cases)**