The code calculates the value of `ans` by adding the product of `k` and `b` to the product of `n - k` and `a`. Since `k` is an integer, `a` and `b` are non-negative integers, and `n` is a non-negative integer, with the constraint `0 <= k <= min(n, b)`, the value of `ans` will be a non-negative integer.

Output State: **ans is a non-negative integer equal to k * b + (n - k) * a, k is an integer, a is a non-negative integer, b is a non-negative integer, n is a non-negative integer, 0 <= k <= min(n, b)**