The code prints the product of `pow` and the result of the expression `2 * (k - tot) - 1`. 

Here, `pow` is 1, `k` is an integer between 1 and 0 inclusive, and `tot` is 0. 

Since `k` is between 1 and 0 inclusive, it can only be 0 or 1. 

If `k` is 0, then `k - tot` is 0 - 0 = 0, and `2 * (k - tot) - 1` is 2 * 0 - 1 = -1. 

If `k` is 1, then `k - tot` is 1 - 0 = 1, and `2 * (k - tot) - 1` is 2 * 1 - 1 = 1.

In both cases, `pow * (2 * (k - tot) - 1)` is 1 * (-1) = -1 or 1 * 1 = 1.

Output: **-1 or 1 (where the value depends on the value of k)**