To calculate the output state, we need to understand the loop's behavior based on the given initial state and the loop's code.

Initial State:
- `size` is 4
- `number` is 10 (not used in the loop)
- `sequence` is [1, 2, 3, 4, 5, 6, 7, 8, 9, 10, 0, 1, 2, 3]
- `result` is returned by `func_1(1, [1, 2, 3, 4, 5, 6, 7, 8, 9, 10, 0, 1, 2, 3])`

Since the function `func_1` is not defined, we'll assume `result` is a value that makes the assertion pass and the loop execute without errors. Let's assume `result` is 10 for this example, as it fits the assertion condition given the initial state of `sequence`.

The loop iterates `size` times (4 times in this case). In each iteration, it modifies the `sequence` list by adding `result` to the element at the index calculated by `-result - i - 1`.

1. First iteration (`i = 0`):
   - Index: `-10 - 0 - 1 = -11`
   - `sequence[-11] += 10`, so `sequence[3]` (since Python uses 0-based indexing and `-11 % 14 = 3`) becomes `4 + 10 = 14`

2. Second iteration (`i = 1`):
   - Index: `-10 - 1 - 1 = -12`
   - `sequence[-12] += 10`, so `sequence[2]` (since `-12 % 14 = 2`) becomes `3 + 10 = 13`

3. Third iteration (`i = 2`):
   - Index: `-10 - 2 - 1 = -13`
   - `sequence[-13] += 10`, so `sequence[1]` (since `-13 % 14 = 1`) becomes `2 + 10 = 12`

4. Fourth iteration (`i = 3`):
   - Index: `-10 - 3 - 1 = -14`
   - `sequence[-14] += 10`, so `sequence[0]` (since `-14 % 14 = 0`) becomes `1 + 10 = 11`

After the loop, `sequence` becomes `[11, 12, 13, 14, 5, 6, 7, 8, 9, 10, 0, 1, 2, 3]`.

Output State: **`size` is 4, `number` is 10, `sequence` is [11, 12, 13, 14, 5, 6, 7, 8, 9, 10, 0, 1, 2, 3], `result` is 10.**