The code prints the value of `n - k + 1` and the value of `1`.

Based on the precondition, `n` is a positive integer (1 ≤ n ≤ 10^18) and `k` is a positive integer (1 ≤ k ≤ 10^18). Additionally, `n` is larger than or equal to `k` and `n` is not equal to `k`. This means that `n - k` will always be a non-negative integer.

The value of `n - k + 1` will be a positive integer greater than or equal to `1`.

The value of `1` is a constant and will always be printed as `1`.

Output: **n - k + 1 (where n - k + 1 is a positive integer greater than or equal to 1), 1**