
Given a Python loop, an initial execution state, and the output states after the first 3 iterations of the loop, determine the output state after all the executions of the loop have finished. 

You must adhere to the text format: Output State: **output state.**

Initial State: T is a positive integer between 1 and 10^4 (inclusive), t is 1, stdin contains multiple lines of input minus two lines that were read, a is a positive integer, b is a positive integer, suma is 0, i is equal to b + 1.
Code of the loop:
for i in range(1, b + 1):
    x = (a - i * (i - 1)) // i ** 2 + 1
    if (a - i * (i - 1)) // i ** 2 + 1 > 0:
        suma += x
        if (a - i * (i - 1)) % i ** 2 == 0 and i * (i - 1) % i ** 2 == 0:
            suma += 1


The output state after the loop executes the first 3 of times includes what needed to be true for the loop to execute at least that number of times:

Output State after the loop executes 1 time: *`T` is a positive integer between 1 and 10^4 (inclusive), `t` is 1, stdin contains multiple lines of input minus two lines that were read, `a` is a positive integer, `b` is at least 1. `suma` is ((a - i * (i - 1)) // i^2) + 1, `i` is 1, `x` is ((a - i * (i - 1)) // i^2) + 1. If ((a - i * (i - 1)) % i^2 == 0 and i * (i - 1) % i^2 == 0), then `suma` is ((a - i * (i - 1)) // i^2) + 2.

**Output State after the loop executes 2 times**: *`T` is a positive integer between 1 and 10^4 (inclusive), `t` is 1, stdin contains multiple lines of input minus two lines that were read, `a` is a positive integer, `b` is at least 2, `i` is 2, `x` is ((a - i * (i - 1)) // i^2) + 1. If ((a - i * (i - 1)) // i^2 + 1 > 0), then if ((a - i * (i - 1)) % i^2 == 0 and i * (i - 1) % i^2 == 0), `suma` is 2 * ((a - i * (i - 1)) // i^2) + 3. Otherwise, `suma` is 2 * ((a - i * (i - 1)) // i^2) + 2.

**Output State after the loop executes 3 times**: *`T` is a positive integer between 1 and 10^4 (inclusive), `t` is 1, stdin contains multiple lines of input minus two lines that were read, `a` is a positive integer, `b` is at least 3, `i` is 3, `x` is ((a - i * (i - 1)) // i^2) + 1. If ((a - i * (i - 1)) // i^2 + 1 > 0), then if ((a - i * (i - 1)) % i^2 == 0 and i * (i - 1) % i^2 == 0), `suma` is 2 * ((a - i * (i - 1)) // i^2) + 3. Otherwise, `suma` is 2 * ((a - i * (i - 1)) // i^2) + 2. If ((a - i * (i - 1)) // i^2 + 1 <= 0), then no changes are made to the variables.




What is the ouput state after the loop executes all the iterations? Change the values of only the variables in the loop head and body.The state of the other variables in the precondition that are not affected by the loop head and body must remain unchanged.
In your response strictly use the format: Output State: **the output state you calculate.**, and describe this output state in Natural language easily understandable by humans.

