The code prints the value of `suma` minus 2, where `suma` is the sum of ((a - i * (i - 1)) // i^2) + 1 for i from 1 to b, and if ((a - i * (i - 1)) % i^2 == 0 and i * (i - 1) % i^2 == 0) for some i, then `suma` is incremented by the number of times this condition is true.
Output: **T is a positive integer between 1 and 10^4 (inclusive), t is 1, stdin contains multiple lines of input minus two lines that were read, a is a positive integer, b is a positive integer, i is equal to b + 1, x is ((a - b * (b - 1)) // b^2) + 1, suma is the sum of ((a - i * (i - 1)) // i^2) + 1 for i from 1 to b. If ((a - i * (i - 1)) % i^2 == 0 and i * (i - 1) % i^2 == 0) for some i, then suma is incremented by the number of times this condition is true, and the value of suma - 2 is being printed**