Postcondition: ***`T` is greater than 0, `t` is 0, `a` is a positive integer, `b` is at least 1, `suma` is equal to `suma + ((a - i * (i - 1)) // i)`, `stdin` contains multiple test cases minus one test case, `i` is 1, and `x` is equal to `(a - i * (i - 1)) // i`. The current value of `i` is such that `((a - i * (i - 1)) % i ** 2 == 0 and i * (i - 1) % i ** 2 == 0)`, meaning that the remainder of `(a - i * (i - 1))` divided by `i` squared is 0, and the remainder of `i * (i - 1)` divided by `i` squared is also 0.***