Let's analyze the code step by step:

1. `sum` is assigned a new value by adding `(i * i - (i - 1) * (i - 1)) * i` to its current value.
2. The current value of `sum` is `1 + (2 * 2 - (2 - 1) * (2 - 1)) * 2`, which simplifies to `1 + (4 - 1) * 2 = 1 + 3 * 2 = 1 + 6 = 7`.
3. The value of `i` is 3.
4. The expression `(i * i - (i - 1) * (i - 1)) * i` evaluates to `(3 * 3 - (3 - 1) * (3 - 1)) * 3 = (9 - 4) * 3 = 5 * 3 = 15`.
5. The new value of `sum` is `7 + 15 = 22`.

The output state is:

**`t` is an integer between 1 and 500 inclusive, `_` is 0, `n` is an integer that must be at least 3, `sum` is 22, `stdin` contains multiple test cases minus one, `i` is 3**

In natural language, the output state is: The value of `sum` has been updated to 22, while the values of `t`, `_`, `n`, `stdin`, and `i` remain unchanged.