Let's break down the code and its impact on the program.

The code is: `sum += (i * i - (i - 1) * (i - 1)) * i`

We know that `i` is 2, so let's substitute this value into the expression:

`sum += (2 * 2 - (2 - 1) * (2 - 1)) * 2`
`sum += (4 - 1) * 2`
`sum += 3 * 2`
`sum += 6`

So, the value of `sum` is incremented by 6.

The initial value of `sum` is 1, so the new value of `sum` is:

`sum = 1 + 6 = 7`

The other variables are not affected by this code.

Therefore, the output state is:

Output State: **`t` is an integer between 2 and 500 inclusive, `_` is 2, `n` is an integer greater than or equal to 3, `sum` is 7, `stdin` contains multiple test cases minus one, `i` is 2, `j` is `n + 1`**

In natural language, the output state is: The value of `sum` has been updated to 7, while all other variables remain unchanged.