Let's break down the code step by step:

1. `sum += (i * i - (i - 1) * (i - 1)) * i`

The value of `sum` is updated by adding the result of the expression `(i * i - (i - 1) * (i - 1)) * i`.

2. Since `i` is 4, we can substitute its value into the expression:

`(4 * 4 - (4 - 1) * (4 - 1)) * 4`
= `(16 - 3 * 3) * 4`
= `(16 - 9) * 4`
= `7 * 4`
= `28`

3. Now, add the result to the initial value of `sum`:

`sum` = `22 + 28`
= `50`

The values of the other variables (`t`, `n`, and `stdin`) are not affected by this code.

Output State: **`t` is at least 1, `n` is at least 5, `sum` is 50, `stdin` contains zero or more inputs: an integer (greater than 0), `i` is 4**

In natural language, the output state is: The values of `t`, `n`, and `stdin` remain unchanged, while the value of `sum` is updated to 50 by adding the result of the expression `(i * i - (i - 1) * (i - 1)) * i` to its initial value. The value of `i` remains 4.