Let's analyze the given code and initial state step by step.

The code is: `sum += (i * i - (i - 1) * (i - 1)) * i`

From the initial state, we know that `i` is 2.

So, let's calculate the expression `(i * i - (i - 1) * (i - 1)) * i`:

`i * i` = 2 * 2 = 4
`(i - 1) * (i - 1)` = (2 - 1) * (2 - 1) = 1 * 1 = 1
`i * i - (i - 1) * (i - 1)` = 4 - 1 = 3
`(i * i - (i - 1) * (i - 1)) * i` = 3 * 2 = 6

Now, let's update the value of `sum`:

`sum` was 1, and we add 6 to it, so `sum` becomes 1 + 6 = 7

The values of the other variables (`n`, `t`, `j`) are not affected by this code.

The stdin still contains zero or more inputs: an integer (greater than 0), as the code does not read from stdin.

Therefore, the output state is:

Output State: **`n` is an integer greater than 1, `i` is 2, `sum` is 7, `t` is at least 3, `j` is `n+1`, stdin contains zero or more inputs: an integer (greater than 0)**