Let's break down the code step by step:

1. `sum += (i * i - (i - 1) * (i - 1)) * i`

The value of `sum` is updated by adding the result of the expression `(i * i - (i - 1) * (i - 1)) * i`.

Since `i` is 3, we can substitute its value into the expression:

`(3 * 3 - (3 - 1) * (3 - 1)) * 3`
= `(9 - 2 * 2) * 3`
= `(9 - 4) * 3`
= `5 * 3`
= `15`

So, `sum` is updated by adding 15 to its current value, which is 7.

Therefore, the new value of `sum` is `7 + 15 = 22`.

The other variables are not affected by this code.

Output State: **`n` is an integer greater than 2, `i` is 3, `sum` is 22, `t` is at least 3, `j` is `n+1`, stdin contains zero or more inputs: an integer (greater than 0)**