The code prints the value of `pow` multiplied by the result of the expression `2 * (k - tot) - 1`. Where `pow` is 1, `k` is an integer (1 <= k <= n), and `tot` is 0.

Output: **`t` is an integer (1 <= t <= 5 * 10^4), `n` is 0, `k` is an integer (1 <= k <= n), `_` is 0, `L` is a list containing at least 1 element which is 0, `stdin` contains t-1 inputs: each of the remaining t-1 inputs is a pair of integers n and k (1 <= k <= n <= 10^9), `tot` is 0, `pow` is 1, `a` is 0. The current value of `tot` is less than `k` and the current value of `k` is less than or equal to the sum of `tot` and `a`, and this is printed: `pow * (2 * (k - tot) - 1)` which is equal to  `1 * (2 * (k - 0) - 1)` which is equal to  `1 * (2 * k - 1)`**