The code prints the result of the expression `pow * (2 * (k - tot) - 1)`. 

Here, `pow` is 2, `tot` is `a` which is the second element in list `L`, and `k` is an integer (1 <= k <= n).

Since the exact value of `a` (the second element in list `L`) and `k` are not provided, we can't compute the exact numerical value of the expression.

However, based on the structure of the problem, the print statement will output the result of the expression `2 * (2 * (k - a) - 1)`, where `a` is the second element in list `L` and `k` is an integer (1 <= k <= n).

Output: **2 * (2 * (k - a) - 1) (where a is the second element in list L and k is an integer (1 <= k <= n))**