The code prints the result of the expression `pow * (2 * (k - tot) - 1)`. Based on the initial state, we can break down the values of the variables involved:

*   `pow` is 1.
*   `k` is an integer between 1 and `n`, but since `n` is 0, `k` must be 1.
*   `tot` is less than `k`, but since `k` is 1, `tot` must be 0.

Substituting these values into the expression, we get:

`1 * (2 * (1 - 0) - 1) = 1 * (2 * 1 - 1) = 1 * (2 - 1) = 1 * 1 = 1`

Therefore, the code will print the value 1.

Output: **1**